src/program_proof/simplepb/apps/clerkpool_proof.v
@@ -1,0 +1,261 @@
+From Perennial.program_proof Require Import grove_prelude.
+From Goose.github_com.mit_pdos.gokv.simplepb.apps Require Import kv.
+From Perennial.program_proof.simplepb Require Import kv_proof.
+From Perennial.program_proof.kv Require Import interface.
+
+Section clerkpool_proof.
+
+Context `{!heapGS Σ, !ekvG Σ}.
+Definition own_ClerkPool c γkv : iProp Σ :=
+  ∃ (cls:list loc) cls_sl,
+  "Hcls" ∷ c ↦[ClerkPool :: "cls"] (slice_val cls_sl) ∗
+  "Hcls_sl" ∷ own_slice cls_sl ptrT 1 (cls) ∗
+  "Hcls_own" ∷ ([∗ list] cl ∈ cls, own_Clerk cl γkv)
+.
+
+Definition is_ClerkPool c γkv : iProp Σ :=
+  ∃ mu (confHost:u64),
+  "#Hmu" ∷ readonly (c ↦[ClerkPool :: "mu"] mu) ∗
+  "#HmuInv" ∷ is_lock nroot mu (own_ClerkPool c γkv) ∗
+  "#HconfHost" ∷ readonly (c ↦[ClerkPool :: "confHost"] #confHost) ∗
+  "#Hhost" ∷ is_kv_config confHost γkv
+.
+
+Lemma wp_doWithClerk c γkv (f:val) Φ :
+  is_ClerkPool c γkv -∗
+  (∀ ck, own_Clerk ck γkv -∗
+  WP f #ck {{ λ _, own_Clerk ck γkv ∗ Φ #() }}) -∗
+  WP ClerkPool__doWithClerk #c f {{ Φ }}
+.
+Proof.
+  iIntros "#Hck HΦ".
+  iNamed "Hck".
+  wp_lam.
+  wp_pures.
+  wp_loadField.
+  wp_apply (acquire_spec with "[$]").
+  iIntros "[Hlocked Hown]".
+  iNamed "Hown".
+  wp_pures.
+  wp_apply wp_ref_of_zero.
+  { done. }
+  iIntros (?) "Hl".
+  wp_pures.
+  wp_loadField.
+  wp_apply (wp_slice_len).
+  wp_if_destruct.
+  {
+    iDestruct (own_slice_sz with "[$]") as %Hsz.
+    wp_loadField.
+    destruct cls.
+    { exfalso. simpl in *. word. }
+    iDestruct (own_slice_small_acc with "Hcls_sl") as "[Hcls_sl Hcls_acc]".
+    wp_apply (wp_SliceGet with "[$Hcls_sl]").
+    { done. }
+    iIntros "Hcls_sl".
+    wp_store.
+    wp_loadField.
+    wp_apply (wp_SliceSkip).
+    { word. }
+    wp_storeField.
+    wp_loadField.
+    iDestruct "Hcls_own" as "[Hcl_own Hcls_own]".
+    iDestruct ("Hcls_acc" with "[$]") as "Hcls_sl".
+    rewrite own_slice_split.
+    iDestruct "Hcls_sl" as "[H1 H2]".
+    iDestruct (slice_small_split _ 1 with "[$]") as "[_ Hcls_sl]".
+    { word. }
+    iDestruct (own_slice_cap_skip _ _ 1 with "[$]") as "?".
+    { word. }
+    rewrite skipn_cons drop_0.
+    wp_apply (release_spec with "[-HΦ Hcl_own Hl]").
+    { iFrame "#∗". iNext. repeat iExists _. iFrame "∗#". }
+    wp_pures.
+    wp_load.
+    wp_bind (f #_).
+    wp_apply (wp_wand with "[HΦ Hcl_own]").
+    { wp_apply ("HΦ"). iFrame. }
+    iIntros (?) "[Hck HΦ]".
+    wp_pures.
+    wp_loadField.
+    iClear "Hhost".
+    clear.
+    wp_apply (acquire_spec with "[$]").
+    iIntros "[Hlocked Hown]".
+    iNamed "Hown".
+    wp_pures.
+    wp_load.
+    wp_loadField.
+    wp_apply (wp_SliceAppend with "[$]").
+    iIntros (?) "Hsl".
+    wp_storeField.
+    wp_loadField.
+    wp_apply (release_spec with "[-HΦ Hl]").
+    { iFrame "#∗". iNext. repeat iExists _. iFrame "∗#". done. }
+    wp_pures.
+    iApply "HΦ".
+  }
+  {
+    wp_loadField.
+    wp_apply (release_spec with "[-HΦ Hl]").
+    { iFrame "#∗". iNext. repeat iExists _. iFrame "∗#". }
+    wp_pures.
+    wp_loadField.
+    wp_apply (wp_MakeClerk with "[$]").
+    iIntros (?) "Hck".
+    wp_store.
+    wp_load.
+    wp_bind (f #_).
+    wp_apply (wp_wand with "[HΦ Hck]").
+    { wp_apply ("HΦ"). iFrame. }
+    iIntros (?) "[Hck HΦ]".
+    wp_pures.
+    wp_loadField.
+    wp_apply (acquire_spec with "[$]").
+    iIntros "[Hlocked Hown]".
+    iNamed "Hown".
+    wp_pures.
+    wp_load.
+    wp_loadField.
+    wp_apply (wp_SliceAppend with "[$]").
+    iIntros (?) "Hsl".
+    wp_storeField.
+    wp_loadField.
+    wp_apply (release_spec with "[-HΦ Hl]").
+    { iFrame "#∗". iNext. repeat iExists _. iFrame "∗#". done. }
+    wp_pures.
+    iApply "HΦ".
+  }
+Qed.
+
+Lemma wp_MakeClerkPool γkv confHost :
+  {{{
+        "#Hhost" ∷ is_kv_config confHost γkv
+  }}}
+    MakeClerkPool #confHost
+  {{{
+        ck, RET #ck; is_ClerkPool ck γkv
+  }}}
+.
+Proof.
+  iIntros (?) "Hpre HΦ".
+  iNamed "Hpre".
+  wp_lam.
+  wp_pures.
+  wp_apply (wp_new_free_lock).
+  iIntros (?) "HmuInv".
+  wp_apply wp_NewSlice.
+  iIntros (?) "Hsl".
+  iApply wp_fupd.
+  wp_apply wp_allocStruct.
+  { val_ty. }
+  iIntros (?) "Hc".
+  iDestruct (struct_fields_split with "Hc") as "HH".
+  iNamed "HH".
+  iMod (readonly_alloc_1 with "mu") as "#Hmu".
+  iMod (readonly_alloc_1 with "confHost") as "#HconfHost".
+  iApply "HΦ".
+  repeat iExists _; iFrame "#".
+  iMod (alloc_lock with "[$] [-]") as "$"; last done.
+  iNext. repeat iExists _; iFrame. rewrite replicate_0. iApply big_sepL_nil. done.
+Qed.
+
+Definition vkvE : coPset := (↑pb_protocol.pbN ∪ ↑clerk_proof.prophReadN ∪ ↑esm_proof.esmN ∪
+                                     ↑stateN).
+Lemma wp_MakeKv γkv confHost :
+  {{{
+        "#Hhost" ∷ is_kv_config confHost γkv
+  }}}
+    MakeKv #confHost
+  {{{
+        k, RET #k; is_Kv k (kv_ptsto γkv) vkvE
+
+  }}}
+.
+Proof.
+  iIntros (?) "Hpre HΦ".
+  iNamed "Hpre".
+  wp_lam.
+  wp_apply (wp_MakeClerkPool with "[$]").
+  iIntros (?) "#Hck".
+  wp_pures.
+  wp_lam. wp_pures.
+  wp_lam. wp_pures.
+  wp_lam. wp_pures.
+  iApply wp_fupd.
+  wp_apply (wp_allocStruct).
+  { val_ty. }
+  iIntros (?) "Hk".
+  iDestruct (struct_fields_split with "Hk") as "HH".
+  iNamed "HH".
+  iApply "HΦ".
+  iMod (readonly_alloc_1 with "Put") as "#?".
+  iMod (readonly_alloc_1 with "Get") as "#?".
+  iMod (readonly_alloc_1 with "ConditionalPut") as "#?".
+  repeat iExists _; iFrame "#".
+  iModIntro.
+  iSplit.
+  {
+    clear Φ.
+    iIntros (?) "* !# * _ Hau".
+    wp_pures.
+    wp_apply (wp_doWithClerk with "[$]").
+    iIntros (?) "Hcl".
+    wp_pures.
+    wp_apply (wp_Clerk__Put with "[$] [Hau]").
+    iNext.
+    unfold vkvE.
+    iMod "Hau" as (?) "[H1 Hau]".
+    iModIntro. iExists _; iFrame.
+    iIntros "H1". iMod ("Hau" with "[$]") as "Hau".
+    iModIntro.
+    iIntros "Hcl".
+    wp_pures. iModIntro.
+    iFrame. wp_pures. by iApply "Hau".
+  }
+  iSplit.
+  {
+    clear Φ.
+    iIntros (?) "* !# * _ Hau".
+    wp_pures.
+    wp_apply (wp_ref_of_zero).
+    { done. }
+    iIntros (?) "Hl".
+    wp_pures.
+    wp_apply (wp_doWithClerk with "[$]").
+    iIntros (?) "Hcl".
+    wp_pures.
+    wp_apply (wp_Clerk__Get with "[$]").
+    unfold vkvE.
+    iMod "Hau" as (?) "[H1 Hau]".
+    iModIntro. iExists _; iFrame.
+    iIntros "H1". iMod ("Hau" with "[$]") as "Hau".
+    iModIntro.
+    iIntros "Hcl".
+    wp_pures. wp_store. iModIntro.
+    iFrame. wp_pures. wp_load. by iApply "Hau".
+  }
+  {
+    clear Φ.
+    iIntros (?) "* !# * _ Hau".
+    wp_pures.
+    wp_apply (wp_ref_of_zero).
+    { done. }
+    iIntros (?) "Hl".
+    wp_pures.
+    wp_apply (wp_doWithClerk with "[$]").
+    iIntros (?) "Hcl".
+    wp_pures.
+    wp_apply (wp_Clerk__CondPut with "[$]").
+    unfold vkvE.
+    iMod "Hau" as (?) "[H1 Hau]".
+    iModIntro. iExists _; iFrame.
+    iIntros "H1". iMod ("Hau" with "[$]") as "Hau".
+    iModIntro.
+    iIntros "Hcl".
+    wp_pures. wp_store. iModIntro.
+    iFrame. wp_pures. wp_load. by iApply "Hau".
+  }
+Qed.
+
+End clerkpool_proof.
